Re-prove match pattern optimization
Included the proofs of optimization rules applied to match patterns to
the more general form of the datatype.
Encountering an issue where termination cannot be proved as described
below.

It's unclear how to say for a generic type classes fixes such as
```isabelle
class T =
	fixes map :: "('a => 'a) => 'a => 'a"
```
How you would express a property about this that allows you to show
termination of mutually recursive calls, e.g.
```isabelle
fun f where "'a::T => 'a"
	"f = map (f)"
```
Since every parameter passed to the mapping function is smaller, e.g.
(map (\lambda x. x) e), x will always be smaller than e,
we know that it will terminate but it is hard to express
this property in Isabelle.

Stratego/CompileRewrite.thy
@@ -97,36 +97,6 @@ value "match_pattern
     (Variable ''y''))
 ''e'' ({|''e''|}, Map.empty)"
 
-
-(*"match v \<langle> ((\<lambda>y. e) \<langle> fresh ''a'') |> descend match_pattern e ''a'')"
-
-fun match_pattern :: "('a::Rewritable) \<Rightarrow> VarName \<Rightarrow> Scope \<Rightarrow> Scope \<times> 'a MATCH" where
-  "match_pattern (UnaryExpr op e) v =
-    match v \<langle>
-      (UnaryPattern op \<langle> fresh ''a'')
-    |> descend match_pattern e ''a''" |
-  "match_pattern (BinaryExpr op e1 e2) v =
-    match v \<langle> 
-      (BinaryPattern op \<langle> fresh ''a'' \<rangle> fresh ''b'')
-    |> descend match_pattern e1 ''a''
-    |> descend match_pattern e2 ''b''" |
-  "match_pattern (ConditionalExpr b e1 e2) v =
-    match v \<langle>
-      (ConditionalPattern \<langle> fresh ''a'' \<rangle> fresh ''b'' \<rangle> fresh ''c'')
-    |> descend match_pattern b ''a''
-    |> descend match_pattern e1 ''b''
-    |> descend match_pattern e2 ''c''" |
-  \<comment> \<open>If a variable is reused, generate an equality check, else, generate a noop.\<close>
-  "match_pattern (VariableExpr vn st) v = 
-    (\<lambda>s. case (snd s) vn of 
-      None \<Rightarrow> (register_name s vn v, noop) |
-      Some v' \<Rightarrow> (register_name s vn v, equality v' v))" |
-  "match_pattern (ConstantExpr c) v =
-    (\<lambda>s. (s, match v (ConstantPattern c)))" |
-  "match_pattern (ConstantVar c) v =
-    (\<lambda>s. (s, match v (ConstantVarPattern c)))" |
-  "match_pattern _ v = (\<lambda>s. (s, noop))"*)
-
 definition gen_pattern :: "('a::Rewritable) \<Rightarrow> VarName \<Rightarrow> 'a MATCH" where
   "gen_pattern p v = snd (match_pattern p v ({|v|}, Map.empty))"
 
@@ -136,12 +106,20 @@ type_synonym 'a Subst = "VarName \<rightharpoonup> 'a"
 fun equal_ignore_vars :: "'a::Rewritable \<Rightarrow> 'a \<Rightarrow> bool" where
   "equal_ignore_vars e1 e2 = ((map_tree (\<lambda>_. var ''a'') e1) = (map_tree (\<lambda>_. var ''a'') e2))"
 
+fun unify :: "string list \<Rightarrow> 'a list \<Rightarrow> 'a Subst \<Rightarrow> 'a Subst option" where
+  "unify [] [] s = Some s" |
+  "unify (v # vs) (e # es) s = 
+    (if s v = Some e then unify vs es s
+     else (if v \<in> dom s \<and> s v \<noteq> Some e then None
+           else unify vs es (s(v \<mapsto> e))))" |
+  "unify _ _ s = None"
+
 fun eval_match :: "('a::Rewritable) MATCH \<Rightarrow> 'a Subst \<Rightarrow> ('a Subst) option" where
   "eval_match (match v e) s =
     (case s v of
       Some e' \<Rightarrow>
         (if equal_ignore_vars e e' then
-          Some (s((List.map (the o varof) (subexprs e)) [\<mapsto>] subexprs e')) else None) |
+          (unify (pattern_variables e) (subexprs e') s) else None) |
       None \<Rightarrow> None)" |
   "eval_match (equality v1 v2) s =
     (if v1 \<in> dom s \<and> v2 \<in> dom s \<and> s v1 = s v2 then Some s else None)" |
@@ -152,64 +130,306 @@ fun eval_match :: "('a::Rewritable) MATCH \<Rightarrow> 'a Subst \<Rightarrow> (
   "eval_match noop s = Some s" |
   "eval_match (condition sc) s = None"
 
-(*
-fun eval_match :: "'a MATCH \<Rightarrow> 'a Subst \<Rightarrow> ('a Subst) option" where
-  "eval_match (match v (UnaryPattern op1 x)) s =
-    (case s v of 
-      Some (UnaryExpr op2 xe) \<Rightarrow>
-        (if op1 = op2 then
-          (if x \<in> dom s then
-            (if s x = Some xe then Some s else None)
-          else Some (s(x\<mapsto>xe)))
-         else None) |
-      Some _ \<Rightarrow> None |
-      None \<Rightarrow> None)" |
-  "eval_match (match v (BinaryPattern op1 x y)) s =
-    (case s v of
-      Some (BinaryExpr op2 xe ye) \<Rightarrow>
-        (if op1 = op2 
-          then 
-          (if x \<in> dom s \<and> s x \<noteq> Some xe then None else 
-          (if y \<in> dom s \<and> s y \<noteq> Some ye then None else 
-          (if x \<in> dom s \<and> y \<in> dom s then Some s else
-          (if x \<in> dom s then Some (s(y\<mapsto>ye)) else
-          (if y \<in> dom s then Some (s(x\<mapsto>xe)) else
-          Some (s(x\<mapsto>xe, y\<mapsto>ye)))))))
-          else None) |
-      Some _ \<Rightarrow> None |
-      None \<Rightarrow> None)" |
-  "eval_match (match v (ConditionalPattern c tb fb)) s =
-    (case s v of
-      Some (ConditionalExpr ce te fe) \<Rightarrow>
-        (if c \<in> dom s \<and> s c \<noteq> Some ce then None else 
-          (if tb \<in> dom s \<and> s tb \<noteq> Some te then None else
-          (if fb \<in> dom s \<and> s fb \<noteq> Some fe then None else 
-          (if c \<in> dom s \<and> tb \<in> dom s \<and> fb \<in> dom s then Some s else
-          (if c \<in> dom s \<and> tb \<in> dom s then Some (s(fb\<mapsto>fe)) else
-          (if c \<in> dom s \<and> fb \<in> dom s then Some (s(tb\<mapsto>te)) else
-          (if tb \<in> dom s \<and> fb \<in> dom s then Some (s(c\<mapsto>ce)) else
-          (if c \<in> dom s then Some (s(tb\<mapsto>te, fb\<mapsto>fe)) else
-          (if tb \<in> dom s then Some (s(c\<mapsto>ce, fb\<mapsto>fe)) else
-          (if fb \<in> dom s then Some (s(c\<mapsto>ce, tb\<mapsto>te)) else
-          Some (s(c\<mapsto>ce, tb\<mapsto>te, fb\<mapsto>fe)))))))))))) |
-      Some _ \<Rightarrow> None |
-      None \<Rightarrow> None)" |
-  "eval_match (match v (ConstantPattern c1)) s =
-    (case s v of 
-      Some (ConstantExpr c2) \<Rightarrow>
-        (if c1 = c2 then Some s else None) |
-      Some _ \<Rightarrow> None |
-      None \<Rightarrow> None)" |
-  "eval_match (equality v1 v2) s =
-    (if v1 \<in> dom s \<and> v2 \<in> dom s \<and> s v1 = s v2 then Some s else None)" |
-  "eval_match (andthen m1 m2) s =
-      (case eval_match m1 s of 
-        None \<Rightarrow> None |
-        Some s' \<Rightarrow> eval_match m2 s')" |
-  "eval_match noop s = Some s" |
-  "eval_match (condition sc) s = (if eval_condition sc then Some s else None)" |
-  "eval_match _ s = None"
-*)
+lemma noop_semantics_rhs:
+  "eval_match (lhs && noop) s = eval_match lhs s"
+  by (simp add: option.case_eq_if)
+
+lemma noop_semantics_lhs:
+  "eval_match (noop && rhs) s = eval_match rhs s"
+  by simp
+
+lemma seq_det_lhs:
+  assumes "\<forall>s. eval_match lhs1 s = eval_match lhs2 s"
+  shows "eval_match (lhs1 && rhs) s = eval_match (lhs2 && rhs) s"
+  using assms by simp
+
+lemma seq_det_rhs:
+  assumes "\<forall>s. eval_match rhs1 s = eval_match rhs2 s"
+  shows "eval_match (lhs && rhs1) s = eval_match (lhs && rhs2) s"
+proof (cases "eval_match lhs s")
+  case None
+  then show ?thesis by simp
+next
+  case (Some a)
+  then obtain s' where s': "eval_match lhs s = Some s'"
+    by simp
+  then have lhs: "eval_match (lhs && rhs1) s = eval_match rhs1 s'"
+    by simp
+  from s' have rhs: "eval_match (lhs && rhs2) s = eval_match rhs2 s'"
+    by simp
+  from lhs rhs show ?thesis using assms
+    by simp
+qed
+
+fun def_vars :: "'a::Rewritable MATCH \<Rightarrow> string set" where
+  "def_vars (match v p) = set (pattern_variables p)" |
+  "def_vars (equality e1 e2) = {e1, e2}" |
+  "def_vars (m1 && m2) = def_vars m1 \<union> def_vars m2" |
+  "def_vars (condition c) = {}" |
+  "def_vars noop = {}"
+
+fun use_vars :: "'a::Rewritable MATCH \<Rightarrow> string set" where
+  "use_vars (match v p) = {v}" |
+  "use_vars (equality e1 e2) = {}" |
+  "use_vars (m1 && m2) = use_vars m1 \<union> (use_vars m2 - def_vars m1)" |
+  "use_vars (condition c) = {}" |
+  "use_vars noop = {}"
+
+fun valid_match :: "'a::Rewritable MATCH \<Rightarrow> bool" where
+  "valid_match (match v e) = (v \<notin> set (pattern_variables e) \<and> distinct (pattern_variables e))" |
+  "valid_match (m1 && m2) = (valid_match m1 \<and> valid_match m2 \<and> use_vars m1 \<inter> def_vars m2 = {})" |
+  "valid_match _ = True"
+
+lemma unify_effect:
+  assumes "unify vs es s = Some a"
+  shows "a = s(vs [\<mapsto>] es)"
+  using assms proof (induction vs es s rule: unify.induct)
+  case (1 s)
+  then show ?case by simp
+next
+  case (2 v vs e es s)
+  then show ?case proof (cases "s v = Some e")
+    case True
+    then show ?thesis
+      by (metis "2.IH"(1) "2.prems" map_upd_triv map_upds_Cons unify.simps(2))
+  next
+    case False
+    then show ?thesis
+      by (metis "2.IH"(2) "2.prems" map_upds_Cons option.distinct(1) unify.simps(2))
+  qed
+next
+  case ("3_1" v va s)
+  then show ?case by simp
+next
+  case ("3_2" v va s)
+  then show ?case by simp
+qed
+
+lemma match_def_affect:
+  assumes "eval_match m u = Some a"
+  shows "\<forall>v. v \<notin> def_vars m \<longrightarrow> u v = a v"
+using assms proof (induction m u arbitrary: a rule: eval_match.induct)
+  case (1 v e s)
+  then show ?case unfolding def_vars.simps pattern_variables.simps eval_match.simps
+    by (smt (verit, best) map_upds_apply_nontin option.case_eq_if option.distinct(1) unify_effect)
+next
+  case (2 v1 v2 s)
+  then show ?case
+    by (metis eval_match.simps(2) option.discI option.inject)
+next
+  case (3 m1 m2 s)
+  then show ?case
+    by (metis (mono_tags, lifting) UnCI def_vars.simps(3) eval_match.simps(3) option.case_eq_if option.collapse)
+next
+  case (4 s)
+  then show ?case
+    by simp
+next
+  case (5 sc s)
+  then show ?case
+    by simp
+qed
+
+lemma use_def:
+  assumes "valid_match m"
+  shows "def_vars m \<inter> use_vars m = {}"
+  using assms apply (induction m)
+  apply simp+
+  apply blast
+  by simp+
+
+lemma match_use_affect:
+  assumes "eval_match m u = Some a"
+  assumes "valid_match m"
+  shows "\<forall>v \<in> use_vars m. u v = a v"
+  using assms apply (induction m u arbitrary: u a rule: eval_match.induct)
+  by (meson disjoint_iff_not_equal match_def_affect use_def)+
+
+
+lemma unify_subset:
+  assumes "unify vs es s = Some a"
+  shows "s \<subseteq>\<^sub>m a"
+using assms proof (induction vs es s rule: unify.induct)
+  case (1 s)
+  then show ?case by simp
+next
+  case (2 v vs e es s)
+  then show ?case proof (cases "s v = Some e")
+    case True
+    then show ?thesis
+      by (metis "2.IH"(1) "2.prems" unify.simps(2))
+  next
+    case False
+    then show ?thesis
+      by (metis "2.IH"(2) "2.prems" fun_upd_None_if_notin_dom map_le_imp_upd_le map_le_refl map_le_trans option.discI unify.simps(2))
+  qed
+next
+  case ("3_1" v va s)
+  then show ?case by simp
+next
+  case ("3_2" v va s)
+  then show ?case by simp
+qed
+
+lemma eval_match_subset:
+  assumes "eval_match m u = Some a"
+  assumes "valid_match m"
+  shows "u \<subseteq>\<^sub>m a"
+  using assms proof (induction m arbitrary: u a)
+  case (match x1 x2)
+  then show ?case using match apply simp
+    using unify.simps(1) unify_subset
+    by (smt (verit, del_insts) option.case_eq_if option.distinct(1))
+next
+  case (equality x1 x2)
+  then show ?case
+    by (metis eval_match.simps(2) map_le_refl option.distinct(1) option.sel)
+next
+  case (andthen m1 m2)
+  then show ?case
+    using valid_match.simps(2)
+    by (metis eval_match.simps(3) map_le_trans option.case_eq_if option.collapse)
+next
+  case (condition x)
+  then show ?case
+    using match_def_affect by fastforce
+next
+  case noop
+  then show ?case by simp
+qed
+
+lemma unify_idempotence:
+  assumes "unify vs es a' = Some a'"
+  assumes "a' \<subseteq>\<^sub>m a"
+  shows "unify vs es a = Some a"
+  using assms proof (induction vs es a' rule: unify.induct)
+  case (1 s)
+  then show ?case by simp
+next
+  case (2 v vs e es s)
+  then show ?case proof (cases "s v = Some e")
+    case True
+    then show ?thesis
+      by (metis "2.IH"(1) "2.prems"(1) "2.prems"(2) domI map_le_def unify.simps(2))
+  next
+    case False
+    then show ?thesis
+      by (metis "2.prems"(1) domIff fun_upd_idem_iff map_le_antisym map_le_imp_upd_le option.discI unify.simps(2) unify_subset)
+  qed
+next
+  case ("3_1" v va s)
+  then show ?case by simp
+next
+  case ("3_2" v va s)
+  then show ?case by simp
+qed
+
+lemma lift_idempotence:
+  assumes "eval_match m a' = Some a'"
+  assumes "a' \<subseteq>\<^sub>m a"
+  assumes "valid_match m"
+  shows "eval_match m a = Some a"
+  using assms proof (induction m arbitrary: a a')
+  case (match x1 x2)
+  then show ?case unfolding eval_match.simps using unify_idempotence
+    by (smt (verit, ccfv_SIG) domIff map_le_def option.case_eq_if option.distinct(1))
+next
+  case (equality x1 x2)
+  from equality show ?case apply simp
+    by (metis domIff map_le_def option.distinct(1))
+next
+  case (andthen m1 m2)
+  obtain a'' where m1eval: "eval_match m1 a' = Some a''"
+    using andthen.prems(1) by fastforce
+  then have m2eval: "eval_match m2 a'' = Some a'"
+    using andthen.prems(1) by auto
+  then have "a'' \<subseteq>\<^sub>m a'"
+    using andthen.prems(3) eval_match_subset valid_match.simps(2) by blast
+  then show ?case
+    by (metis andthen.IH(1) andthen.IH(2) andthen.prems(2) andthen.prems(3) eval_match.simps(3) eval_match_subset m1eval m2eval map_le_antisym option.simps(5) valid_match.simps(2))
+next
+  case (condition x)
+  then show ?case
+    by (metis eval_match.simps(5) option.distinct(1))
+next
+  case noop
+  then show ?case by simp
+qed
+
+lemma idempotent_unify2:
+  assumes "unify vs es u = Some a"
+  shows "unify vs es a = Some a"
+using assms proof (induction vs es u rule: unify.induct)
+  case (1 s)
+  then show ?case by simp
+next
+  case (2 v vs e es s)
+  then show ?case proof (cases "s v = Some e")
+    case True
+    then show ?thesis
+      by (metis "2.IH"(1) "2.prems" domI map_le_def unify.simps(2) unify_subset)
+  next
+    case False
+    then show ?thesis
+      by (metis (no_types, lifting) "2.IH"(2) "2.prems" domI fun_upd_same map_le_def option.distinct(1) unify.simps(2) unify_subset)
+  qed
+next
+  case ("3_1" v va s)
+  then show ?case by simp
+next
+  case ("3_2" v va s)
+  then show ?case by simp
+qed
+
+lemma idempotent_match:
+  assumes "eval_match m u = Some a"
+  assumes "valid_match m"
+  shows "eval_match m a = Some a"
+  using assms 
+proof (induction m arbitrary: u a)
+  case (match x1 x2)
+  then show ?case using idempotent_unify2
+    by (smt (verit) def_vars.simps(1) eval_match.simps(1) match_def_affect option.case_eq_if valid_match.simps(1))
+next
+  case (equality x1 x2)
+  then show ?case
+    by (metis (no_types, lifting) eval_match.simps(2) eval_match_subset lift_idempotence)
+next
+  case (andthen m1 m2)
+  obtain a' where m1eval: "eval_match m1 u = Some a'"
+    using andthen.prems(1) by fastforce
+  have m1idem: "eval_match m1 a' = Some a'"
+    using andthen.IH(1) andthen.prems(2) m1eval valid_match.simps(2) by blast
+  have validm1: "valid_match m1"
+    using andthen.prems(2) by auto
+  have m2eval: "eval_match m2 a' = Some a"
+    using andthen.prems(1) m1eval by auto
+  have validm2: "valid_match m2"
+    using andthen.prems(2) by auto
+  have m2idem: "eval_match m2 a = Some a"
+    using m2eval validm2
+    using andthen.IH(2) by blast
+  have "a' \<subseteq>\<^sub>m a"
+    using eval_match_subset m2eval validm2 by blast
+  then have "eval_match m1 a = Some a"
+    using m1idem lift_idempotence validm1 by blast
+  then show ?case
+    by (simp add: m2idem)
+next
+  case (condition x)
+  then show ?case
+    by (metis eval_match.simps(5))
+next
+  case noop
+  then show ?case
+    by simp
+qed     
+
+lemma match_eq:
+  assumes "valid_match m"
+  shows "eval_match (m && m) u = eval_match m u"
+  using assms
+  by (simp add: idempotent_match option.case_eq_if)
 
 
 subsection \<open>Combining Rules\<close>
@@ -221,6 +441,13 @@ datatype 'a Rules =
   seq "'a Rules" "'a Rules" (infixl "\<then>" 49) |
   choice "('a Rules) list"
 
+fun valid_rules :: "'a::Rewritable Rules \<Rightarrow> bool" where
+  "valid_rules (m ? r) = (valid_match m \<and> valid_rules r)" |
+  "valid_rules (r1 else r2) = (valid_rules r1 \<and> valid_rules r2)" |
+  "valid_rules (r1 \<then> r2) = (valid_rules r1 \<and> valid_rules r2)" |
+  "valid_rules (choice rules) = (\<forall>r \<in> set rules. valid_rules r)" |
+  "valid_rules _ = True"
+
 function ground_expr :: "'a::Rewritable \<Rightarrow> Scope \<Rightarrow> 'a" where
   "ground_expr e (s, m) =
     (case varof e of
@@ -230,40 +457,8 @@ function ground_expr :: "'a::Rewritable \<Rightarrow> Scope \<Rightarrow> 'a" wh
   apply auto[1]
   by fastforce
 
+(* Requires a proof that all the arguments to the map tree anonymous function are less than the original input *)
 termination ground_expr sorry
-(*
-    UnaryExpr op (ground_expr e s)" |
-  "ground_expr (BinaryExpr op e1 e2) s = 
-    BinaryExpr op (ground_expr e1 s) (ground_expr e2 s)" |
-  "ground_expr (ConditionalExpr b e1 e2) s = 
-    ConditionalExpr (ground_expr b s) (ground_expr e1 s) (ground_expr e2 s)" |
-  "ground_expr (VariableExpr vn st) (s, m) = 
-    (case m vn of None \<Rightarrow> VariableExpr vn st 
-                | Some v' \<Rightarrow> VariableExpr v' st)" |
-  "ground_expr e s = e"*)
-
-(*fun ground_result :: "Result \<Rightarrow> Scope \<Rightarrow> Result" where
-  "ground_result (ExpressionResult e) s = ExpressionResult (ground_expr e s)" |
-  "ground_result (forZero e) s = forZero (ground_expr e s)"
-
-fun ground_condition :: "SideCondition \<Rightarrow> Scope \<Rightarrow> SideCondition" where
-  "ground_condition (IsConstantExpr p) s = (IsConstantExpr (ground_expr p s))" |
-  "ground_condition (IsIntegerStamp p) s = (IsIntegerStamp (ground_expr p s))" |
-  "ground_condition (IsBoolStamp p) s = (IsBoolStamp (ground_expr p s))" |
-  "ground_condition (WellFormed st) s = (WellFormed st)" |
-  "ground_condition (IsStamp e st) s = (IsStamp (ground_expr e s) st)" |
-  "ground_condition (IsConstantValue e s' v) s = (IsConstantValue (ground_expr e s) (ground_expr s' s) v)" |
-  "ground_condition (AlwaysDistinct e1 e2) s = (AlwaysDistinct (ground_expr e1 s) (ground_expr e2 s))" |
-  "ground_condition (NeverDistinct e1 e2) s = (NeverDistinct (ground_expr e1 s) (ground_expr e2 s))" |  
-  "ground_condition (StampUnder e1 e2) s = (StampUnder (ground_expr e1 s) (ground_expr e2 s))" |
-  "ground_condition (UpMaskEquals e m) s = (UpMaskEquals (ground_expr e s) m)" |
-  "ground_condition (DownMaskEquals e m) s = (DownMaskEquals (ground_expr e s) m)" |
-  "ground_condition (UpMaskCancels e1 e2) s = (UpMaskCancels (ground_expr e1 s) (ground_expr e2 s))" |
-  "ground_condition (PowerOf2 e) s = (PowerOf2 (ground_expr e s))" |
-  "ground_condition (IsBool e) s = (IsBool (ground_expr e s))" |
-  "ground_condition (And sc1 sc2) s = And (ground_condition sc1 s) (ground_condition sc2 s)" |
-  "ground_condition (Not sc) s = Not (ground_condition sc s)" |
-  "ground_condition (Empty) s = Empty"*)
 
 fun generate :: "'a::Rewritable \<Rightarrow> 'a \<Rightarrow> 'a \<Rightarrow> 'a Rules" where
   "generate p r sc = 
@@ -271,12 +466,10 @@ fun generate :: "'a::Rewritable \<Rightarrow> 'a \<Rightarrow> 'a \<Rightarrow> 
      in ((m && condition (ground_expr sc s)) ? (base (ground_expr r s))))"
 
 subsubsection \<open>Rules Semantics\<close>
-definition start_unification where
-  "start_unification e = ((\<lambda>x. None)(STR ''e'' := Some e))"
 
 text \<open>Replace any variable expressions with value in a substitution.\<close>
 fun evaluated_terms where
-  "evaluated_terms f es s = (List.map (\<lambda>e. f e s) es)"
+  "evaluated_terms f es s = map (\<lambda>e. f e s) es"
 
 fun has_none :: "('a option) list \<Rightarrow> bool" where
   "has_none [] = False" |
@@ -293,33 +486,6 @@ function eval_expr :: "'a::Rewritable \<Rightarrow> 'a Subst \<Rightarrow> 'a op
   by fastforce+
 
 termination eval_expr sorry
-
-(*
-  "eval_expr (UnaryExpr op e) u = (case (eval_expr e u)
-    of None \<Rightarrow> None | Some e' \<Rightarrow> Some (UnaryExpr op e'))" |
-  "eval_expr (BinaryExpr op e1 e2) u = (case (eval_expr e1 u)
-    of None \<Rightarrow> None | Some e1' \<Rightarrow> 
-    (case (eval_expr e2 u)
-      of None \<Rightarrow> None | Some e2' \<Rightarrow> Some (BinaryExpr op e1' e2')))" |
-  "eval_expr (ConditionalExpr e1 e2 e3) u = (case (eval_expr e1 u)
-    of None \<Rightarrow> None | Some e1' \<Rightarrow>
-    (case (eval_expr e2 u)
-      of None \<Rightarrow> None | Some e2' \<Rightarrow>
-        (case (eval_expr e2 u)
-          of None \<Rightarrow> None | Some e3' \<Rightarrow> Some (ConditionalExpr e1' e2' e3'))))" |
-  "eval_expr e u = Some e"
-
-
-fun eval_result :: "Result \<Rightarrow> Subst \<Rightarrow> IRExpr option" where
-  "eval_result (ExpressionResult e) s = (eval_expr e s)" |
-  "eval_result (forZero e) s = (case eval_expr e s of
-    None \<Rightarrow> None |
-    Some r \<Rightarrow> Some (ConstantExpr (IntVal (stp_bits (stamp_expr r)) 0)))"
-
-lemma remove1_size:
-  "x \<in> set xs \<Longrightarrow> size (remove1 x xs) < size xs"
-  by (metis diff_less length_pos_if_in_set length_remove1 zero_less_one)
-*)
 
 inductive eval_rules :: "('a::Rewritable) Rules \<Rightarrow> 'a Subst \<Rightarrow> 'a option \<Rightarrow> bool" where
   \<comment> \<open>Evaluate the result\<close>
@@ -356,15 +522,201 @@ inductive eval_rules :: "('a::Rewritable) Rules \<Rightarrow> 'a Subst \<Rightar
     eval_rules r2 u r\<rbrakk>
    \<Longrightarrow> eval_rules (r1 \<then> r2) u r"
 
+inductive_cases baseE: "eval_rules (base e') u e"
+inductive_cases condE: "eval_rules (cond m r) u e"
+inductive_cases elseE: "eval_rules (r1 else r2) u e"
+inductive_cases choiceE: "eval_rules (choice r) u e"
+inductive_cases seqE: "eval_rules (r1 \<then> r2) u e"
 
+code_pred [show_modes] eval_rules .
 
+lemma choice_join:
+  assumes "eval_rules (a) u e = eval_rules (f a) u e"
+  assumes "eval_rules (choice rules) u e = eval_rules (choice (map f rules)) u e"
+  shows "eval_rules (choice (a # rules)) u e = eval_rules (choice (map f (a # rules))) u e"
+  using assms
+  by (smt (verit, ccfv_threshold) choiceE eval_rules.intros(6) eval_rules.intros(7) list.map_disc_iff list.set_intros(1) list.set_intros(2) list.simps(9) option.distinct(1) set_ConsD)
 
+lemma chain_equiv:
+  "eval_rules (m1 ? (m2 ? r)) u e = eval_rules ((m1 && m2) ? r) u e"
+  using condE apply auto[1]
+   apply (smt (verit, best) condE eval_match.simps(3) eval_rules.intros(2) eval_rules.intros(3) option.simps(4) option.simps(5))
+  by (metis (no_types, lifting) condE eval_match.simps(3) eval_rules.intros(2) eval_rules.intros(3) is_none_code(2) is_none_simps(1) option.case_eq_if option.collapse)
 
+lemma eval_choice: "{e. eval_rules (choice rules) u e \<and> e \<noteq> None} = {e | e r . r \<in> set rules \<and> eval_rules r u e \<and> e \<noteq> None}"
+  using choiceE eval_rules.intros(6) by fastforce
 
+lemma eval_choice_none: "eval_rules (choice rules) u None = (\<forall> r \<in> set rules . eval_rules r u None)"
+  by (metis choiceE eval_rules.intros(7) length_pos_if_in_set list.size(3) nless_le option.distinct(1))
 
+inductive_cases evalRulesE: "eval_rules r u e"
 
+lemma eval_always_result:
+  "\<exists> e. eval_rules r u e"
+  apply (induction r arbitrary: u)
+  using eval_rules.intros(1) apply auto[1]
+  using eval_rules.intros(2,3) apply (metis option.exhaust)
+  using eval_rules.intros(4,5) apply (metis split_option_ex) 
+  using eval_rules.intros(9,10) apply (metis split_option_ex) 
+  using eval_rules.intros(6,7) by (metis split_option_ex) 
 
+lemma unordered_choice:
+  assumes "set rules = set rules'"
+  shows "\<forall>e. eval_rules (choice rules) u e = eval_rules (choice rules') u e"
+  using assms by (metis choiceE eval_choice_none eval_rules.intros(6))
 
+lemma monotonic_cond:
+  assumes "\<forall>e u. eval_rules r u e = eval_rules (f r) u e"
+  shows "\<forall>e u. eval_rules (m ? r) u e = eval_rules (m ? f r) u e"
+  using assms by (metis condE eval_rules.intros(2) eval_rules.intros(3))
+
+lemma monotonic_else:
+  assumes "\<forall>e u. eval_rules r1 u e = eval_rules (f r1) u e"
+  assumes "\<forall>e u. eval_rules r2 u e = eval_rules (f r2) u e"
+  shows "\<forall>e. eval_rules (r1 else r2) u e = eval_rules (f r1 else f r2) u e"
+  using assms
+  by (smt (verit, best) elseE eval_rules.intros(4) eval_rules.intros(5))
+
+lemma monotonic_seq:
+  assumes "\<forall>e u. eval_rules r1 u e = eval_rules (f r1) u e"
+  assumes "\<forall>e u. eval_rules r2 u e = eval_rules (f r2) u e"
+  shows "\<forall>e. eval_rules (r1 \<then> r2) u e = eval_rules (f r1 \<then> f r2) u e"
+  using assms
+  by (smt (verit) eval_rules.simps seqE)
+
+lemma monotonic_choice:
+  assumes "\<forall>r e u. r \<in> set rules \<longrightarrow> eval_rules r u e = eval_rules (f r) u e"
+  shows "\<forall>e. eval_rules (choice rules) u e = eval_rules (choice (map f rules)) u e"
+  using assms apply (induction rules) apply simp
+  by (metis choice_join list.set_intros(1) list.set_intros(2))
+
+lemmas monotonic =
+  monotonic_cond
+  monotonic_else
+  monotonic_choice
+  monotonic_seq
+
+lemma map_None:
+  "(\<forall>r\<in>set rules. eval_rules (m ? r) u None) = eval_rules (choice (map ((?) m) rules)) u None"
+  (is "?lhs = eval_rules ?rhs u None")
+proof -
+  have setequiv: "set (map ((?) m) rules) = {m ? r | r . r\<in>set rules}"
+    by (simp add: Setcompr_eq_image)
+  then show ?thesis
+    using eval_choice_none
+    by fastforce
+qed
+
+lemma setequiv: "set (map ((?) m) rules) = {m ? r | r . r\<in>set rules}"
+  by (simp add: Setcompr_eq_image)
+
+lemma pull_cond_out_rhs:
+  assumes "eval_rules (choice (map ((?) m) rules)) u e" (is "eval_rules ?lhs u e")
+  shows "eval_rules (m ? choice rules) u e" (is "eval_rules ?rhs u e")
+  proof (cases "eval_match m u")
+    case None \<comment> \<open>If m doesn't match then both the lhs and rhs should evaluate to e = None\<close>
+    have lhs: "\<forall>e. eval_rules ?lhs u e \<longrightarrow> e = None"
+      using None eval_rules.intros(3) eval_rules.intros(7)
+      by (smt (verit, del_insts) choiceE condE ex_map_conv option.distinct(1))
+    have rhs: "\<forall>e. eval_rules ?rhs u e \<longrightarrow> e = None"
+      by (metis None condE option.distinct(1))
+    then show ?thesis using lhs rhs
+      using eval_always_result
+      using assms by blast
+  next
+    case match: (Some a) \<comment> \<open>Drop down into evaluation post matching m\<close>
+      have allEval: "\<forall>r \<in> set rules. eval_rules r a e = eval_rules (m ? r) u e"
+        by (metis match condE eval_rules.intros(2) option.distinct(1) option.sel)
+        then show ?thesis
+        proof (cases e)
+          case evalsNone: None
+          have "\<forall>r \<in> set rules. eval_rules r a None"
+            using evalsNone allEval assms map_None by blast
+          then have "\<forall>r \<in> set rules. eval_rules (m ? r) u None"
+            using evalsNone allEval by blast
+          then have "eval_rules ?lhs u None"
+            by (simp add: map_None)
+          then show ?thesis
+            using evalsNone
+            using \<open>\<forall>r\<in>set rules. eval_rules r a None\<close> eval_choice_none eval_rules.intros(2) match by blast
+        next
+          case evalsSome: (Some a')
+            then have "\<exists>r \<in> set rules. eval_rules (m ? r) u (Some a')"
+              using condE assms match
+              using choiceE by fastforce
+            then have "\<exists>r \<in> set rules. eval_rules (m ? r) u e"
+              by (simp add: evalsSome)
+            then have "eval_rules ?rhs u e"
+              using allEval eval_rules.intros(2) eval_rules.intros(6) evalsSome match by blast
+            then show ?thesis
+              by simp
+          qed
+        qed
+
+lemma pull_cond_out_lhs:
+  assumes "eval_rules (m ? choice rules) u e" (is "eval_rules ?lhs u e")
+  shows "eval_rules (choice (map ((?) m) rules)) u e" (is "eval_rules ?rhs u e")
+  proof (cases "eval_match m u")
+    case None \<comment> \<open>If m doesn't match then both the lhs and rhs should evaluate to e = None\<close>
+    have lhs: "\<forall>e. eval_rules ?lhs u e \<longrightarrow> e = None"
+      using None eval_rules.intros(3) eval_rules.intros(7)
+      by (smt (verit, del_insts) choiceE condE ex_map_conv option.distinct(1))
+    have rhs: "\<forall>e. eval_rules ?rhs u e \<longrightarrow> e = None"
+      by (simp add: lhs pull_cond_out_rhs)
+    then show ?thesis using lhs rhs
+      using eval_always_result
+      using assms by blast
+  next
+    case match: (Some a) \<comment> \<open>Drop down into evaluation post matching m\<close>
+      have allEval: "\<forall>r \<in> set rules. eval_rules r a e = eval_rules (m ? r) u e"
+        by (metis match condE eval_rules.intros(2) option.distinct(1) option.sel)
+        then show ?thesis
+        proof (cases e)
+          case evalsNone: None
+          have "\<forall>r \<in> set rules. eval_rules r a None"
+            by (metis assms condE eval_choice_none evalsNone match option.discI option.inject)
+          then have "\<forall>r \<in> set rules. eval_rules (m ? r) u None"
+            using evalsNone allEval by blast
+          then show ?thesis
+            using evalsNone map_None by blast
+        next
+          case evalsSome: (Some a')
+            then have "\<exists>r \<in> set rules. eval_rules (m ? r) u (Some a')"
+              using condE assms match
+              using choiceE
+              by (metis allEval option.distinct(1) option.sel)
+            then have "\<exists>r \<in> set rules. eval_rules (m ? r) u e"
+              by (simp add: evalsSome)
+            then have "eval_rules ?rhs u e"
+              by (metis eval_rules.intros(6) evalsSome image_eqI image_set)
+            then show ?thesis
+              by simp
+          qed
+        qed
+
+lemma pull_cond_out:
+  "eval_rules (choice (map ((?) m) rules)) u e = eval_rules (m ? choice rules) u e"
+  using pull_cond_out_lhs pull_cond_out_rhs by blast
+
+lemma choice_Single:
+  "eval_rules (choice [r]) u e = eval_rules r u e"
+  apply (cases e)
+  using eval_choice_none apply auto[1]
+  using choiceE eval_rules.intros(6) apply fastforce apply fastforce
+  by (smt (verit, best) choiceE eval_rules.intros(6) list.set_cases list.set_intros(1) neq_Nil_conv set_ConsD)
+
+lemma redundant_conditions:
+  assumes "valid_match m"
+  shows "eval_rules (m ? (m ? r1)) u e = eval_rules (m ? r1) u e" (is "?lhs = ?rhs")
+proof -
+  have "?lhs = eval_rules ((m && m) ? r1) u e"
+    using chain_equiv
+    by blast
+  moreover have "eval_rules ((m && m) ? r1) u e = ?rhs"
+    using match_eq sledgehammer
+    by (smt (verit) Rules.distinct(1) Rules.distinct(11) Rules.distinct(13) Rules.distinct(9) Rules.inject(2) assms eval_rules.simps)
+  ultimately show ?thesis by simp
+qed
 
 subsection \<open>Rule Optimization\<close>
 
@@ -374,6 +726,15 @@ fun elim_noop :: "'a MATCH \<Rightarrow> 'a MATCH" where
   "elim_noop (lhs && rhs) = ((elim_noop lhs) && (elim_noop rhs))" |
   "elim_noop m = m"
 
+lemma sound_optimize_noop:
+  "eval_match m s = eval_match (elim_noop m) s"
+  apply (induction m arbitrary: s rule: elim_noop.induct)
+  using noop_semantics_rhs apply force+
+  using seq_det_rhs
+  apply (metis elim_noop.simps(14) elim_noop.simps(22)) apply force
+  apply (metis elim_noop.simps(16) seq_det_lhs seq_det_rhs)
+  by simp+
+
 fun eliminate_noop :: "'a::Rewritable Rules \<Rightarrow> 'a Rules" where
   "eliminate_noop (base e) = base e" |
   "eliminate_noop (m ? r) = elim_noop m ? eliminate_noop r" |
@@ -381,6 +742,33 @@ fun eliminate_noop :: "'a::Rewritable Rules \<Rightarrow> 'a Rules" where
   "eliminate_noop (choice rules) = choice (List.map eliminate_noop rules)" |
   "eliminate_noop (r1 \<then> r2) = (eliminate_noop r1 \<then> eliminate_noop r2)"
 
+lemma eliminate_noop_valid:
+  "eval_rules r u e = eval_rules (eliminate_noop r) u e"
+  apply (induction r arbitrary: u e rule: eliminate_noop.induct)
+  apply simp
+  using eliminate_noop.simps(2) condE sound_optimize_noop
+    apply (smt (verit) eval_rules.simps) 
+  using eliminate_noop.simps(3) elseE
+   apply (smt (verit, del_insts) eval_rules.intros(4) eval_rules.intros(5))
+  unfolding eliminate_noop.simps(4)
+  subgoal premises ind for rules u e 
+    using ind apply (induction rules) apply simp
+    subgoal premises ind' for a rules'
+    proof -
+      have a: "eval_rules (a) u e = eval_rules (eliminate_noop a) u e"
+        using ind' by simp
+      have rules: "eval_rules (choice rules') u e = eval_rules (choice (map eliminate_noop rules')) u e"
+        using ind' by auto
+      have "eval_rules (choice (a # rules')) u e = eval_rules (choice (map eliminate_noop (a # rules'))) u e"
+        using a rules using choice_join
+        by blast
+      then show ?thesis by simp
+    qed
+    done
+  by (smt (verit) Rules.distinct(11) Rules.distinct(15) Rules.distinct(19) Rules.distinct(5) Rules.inject(4) eliminate_noop.simps(5) eval_rules.simps)
+
+
+(*
 fun elim_empty :: "'a MATCH \<Rightarrow> 'a MATCH" where
   "elim_empty (condition Empty) = noop" |
   "elim_empty (m1 && m2) = (elim_empty m1 && elim_empty m2)" |
@@ -391,10 +779,8 @@ fun eliminate_empty :: "'a::Rewritable Rules \<Rightarrow> 'a Rules" where
   "eliminate_empty (m ? r) = elim_empty m ? eliminate_empty r" |
   "eliminate_empty (r1 else r2) = (eliminate_empty r1 else eliminate_empty r2)" |
   "eliminate_empty (choice rules) = choice (List.map eliminate_empty rules)" |
-  "eliminate_empty (r1 \<then> r2) = (eliminate_empty r1 \<then> eliminate_empty r2)"
+  "eliminate_empty (r1 \<then> r2) = (eliminate_empty r1 \<then> eliminate_empty r2)"*)
 
-
-notation plus (infixl "+" 65)
 fun combined_size :: "'a::Rewritable Rules \<Rightarrow> nat" where
   "combined_size (m ? r) = (2 * size m) + combined_size r" |
   "combined_size (base e) = 0" |
@@ -402,11 +788,10 @@ fun combined_size :: "'a::Rewritable Rules \<Rightarrow> nat" where
   "combined_size (choice (rule # rules)) = 1 + combined_size rule + combined_size (choice rules)" |
   "combined_size (choice []) = 1" |
   "combined_size (r1 \<then> r2) = combined_size r1 + combined_size r2"
-no_notation plus (infixl "+" 65)
 
 function (sequential) lift_match :: "'a::Rewritable Rules \<Rightarrow> 'a Rules" where
   "lift_match (r1 else r2) = ((lift_match r1) else (lift_match r2))" |
-  "lift_match (choice rules) = choice (List.map lift_match rules)" |
+  "lift_match (choice rules) = choice (map lift_match rules)" |
   "lift_match ((m1 && m2) ? r) = (lift_match (m1 ? (m2 ? r)))" |
   "lift_match (m ? r) = m ? (lift_match r)" |
   "lift_match (base e) = (base e)" |
@@ -416,10 +801,30 @@ termination lift_match
   apply (relation "measures [combined_size, size]") apply auto[1]
   apply auto[1] apply auto[1] apply simp
   subgoal for rules x apply (induction rules) apply simp by fastforce
-  apply simp subgoal for m2 r apply (cases m2) sorry
-        apply simp+
-  apply blast
-  by auto
+  apply simp subgoal for m2 r apply (cases m2)
+    apply auto[1]
+    by simp+
+  by fastforce+
+
+lemma lift_match_valid:
+  "eval_rules r u e = eval_rules (lift_match r) u e"
+  apply (induction r arbitrary: u e rule: lift_match.induct) 
+           apply simp 
+  using lift_match.simps(1) elseE
+  apply (smt (verit, ccfv_threshold) eval_rules.intros(4) eval_rules.intros(5))
+  unfolding lift_match.simps(2)
+  subgoal premises ind for rules u e 
+    using ind apply (induction rules) apply simp
+    using choice_join
+    by (metis list.set_intros(1) list.set_intros(2))
+        apply (simp add: chain_equiv)
+       apply (metis condE eval_rules.intros(2) eval_rules.intros(3) lift_match.simps(4))
+        apply (metis condE eval_rules.intros(2) eval_rules.intros(3) lift_match.simps(5))
+       apply (metis condE eval_rules.intros(2) eval_rules.intros(3) lift_match.simps(6))
+      apply (metis condE eval_rules.intros(2) eval_rules.intros(3) lift_match.simps(7))
+    apply simp
+  by (smt (verit) Rules.distinct(11) Rules.distinct(15) Rules.distinct(19) Rules.distinct(5) Rules.inject(4) eval_rules.simps lift_match.simps(9))
+
 
 fun join_conditions :: "'a::Rewritable Rules \<Rightarrow> 'a Rules option" where
   "join_conditions (m1 ? r1 else m2 ? r2) = 
@@ -429,6 +834,29 @@ fun join_conditions :: "'a::Rewritable Rules \<Rightarrow> 'a Rules option" wher
     (if m1 = m2
       then Some ((m1 ? r1)) else None)" |
   "join_conditions r = None"
+
+lemma join_conditions_shrinks:
+  "join_conditions r = Some r' \<Longrightarrow> (<) (size r') (size r)"
+  apply (induction r rule: join_conditions.induct)
+  using Rules.size(7) Rules.size(8) Suc_le_eq add.left_commute add.right_neutral antisym_conv1 join_conditions.simps(1) le_simps(1) option.distinct(1) option.sel plus_nat.simps(2)
+   add_Suc_right le_add2
+  apply (smt (z3))
+  apply (metis Rules.size(7) add.right_neutral add_Suc_right join_conditions.simps(2) less_add_Suc2 option.distinct(1) option.sel)
+  by simp+
+
+lemma join_conditions_valid:
+  assumes "valid_rules r"
+  shows "join_conditions r = Some r' \<Longrightarrow> eval_rules r u e = eval_rules r' u e"
+  using assms apply (induction r rule: join_conditions.induct)
+  apply (smt (verit, ccfv_threshold) condE elseE eval_rules.intros(2) eval_rules.intros(3) eval_rules.intros(4) eval_rules.intros(5) join_conditions.simps(1) option.distinct(1) option.sel)
+  subgoal premises p for m1 m2 r
+  proof -
+    have v1:"valid_match m1" using p(2) by simp
+    moreover have v2:"valid_match m2" using p(2) by simp
+    ultimately show ?thesis
+      by (metis join_conditions.simps(2) option.discI option.sel p(1) redundant_conditions)
+  qed
+  by simp+
 
 function lift_common :: "'a::Rewritable Rules \<Rightarrow> 'a Rules" where
   "lift_common (r1 else r2) = (
@@ -448,9 +876,61 @@ function lift_common :: "'a::Rewritable Rules \<Rightarrow> 'a Rules" where
 termination
   apply (relation "measures [size]") apply auto[1]
     apply simp subgoal for r1 r2 apply (induction r1 rule: join_conditions.induct) by simp+
-   apply auto[1] sorry
+   apply auto[1]
+  using join_conditions_shrinks apply fastforce+
+  by (simp add: le_imp_less_Suc size_list_estimation')+
 
-notation plus (infixl "+" 65)
+lemma lift_common_valid:
+  assumes "valid_rules r"
+  shows "eval_rules r u e = eval_rules (lift_common r) u e"
+  using assms proof (induction r arbitrary: u e rule: lift_common.induct)
+  case (1 r1 r2)
+  then show ?case
+  proof (cases "join_conditions (r1 else r2)")
+    case None
+    then have "(lift_common (r1 else r2)) = (lift_common r1 else lift_common r2)"
+      by simp
+    then show ?thesis using 1
+      by (simp add: None monotonic_else)
+  next
+    case (Some a)
+    then obtain m1 m2 r1' r2' where ex: "(r1 else r2) = (m1 ? r1' else m2 ? r2')"
+      by (smt (z3) Rules.distinct(9) join_conditions.elims option.distinct(1))
+    then have "m1 = m2"
+      by (metis Some join_conditions.simps(1) option.distinct(1))
+    then show ?thesis using 1
+      using ex join_conditions_valid
+      by (metis (no_types, lifting) join_conditions.simps(1) lift_common.simps(1) option.case_eq_if option.distinct(1) option.sel valid_rules.simps(1) valid_rules.simps(2))
+  qed
+next
+  case (2 m r)
+  then show ?case
+  proof (cases "join_conditions (m ? r)")
+    case None
+    then have "(lift_common (m ? r)) = (m ? lift_common r)"
+      by simp
+    then show ?thesis using 2
+      by (simp add: None monotonic_cond)
+  next
+    case (Some a)
+    then obtain m1 m2 r' where ex: "(m ? r) = (m1 ? (m2 ? r'))"
+      by (smt (z3) Rules.distinct(9) join_conditions.elims option.distinct(1))
+    then have "m1 = m2"
+      by (metis Some join_conditions.simps(2) option.distinct(1))
+    then show ?thesis using 2
+      by (simp add: ex join_conditions_valid)
+  qed
+next
+  case (3 rules)
+  then show ?case by (simp add: monotonic_choice)
+next
+  case (4 e)
+  then show ?case by simp
+next
+  case (5 r1 r2)
+  then show ?case by (simp add: monotonic_seq)
+qed
+
 fun common_size :: "'a::Rewritable Rules \<Rightarrow> nat" where
   "common_size (m ? r) = 1 + common_size r" |
   "common_size (base e) = 0" |
@@ -458,7 +938,6 @@ fun common_size :: "'a::Rewritable Rules \<Rightarrow> nat" where
   "common_size (choice (rule # rules)) = 1 + common_size rule + common_size (choice rules)" |
   "common_size (choice []) = 0" |
   "common_size (r1 \<then> r2) = 1 + common_size r1 + common_size r2"
-no_notation plus (infixl "+" 65)
 
 fun find_common :: "'a::Rewritable MATCH \<Rightarrow> 'a Rules \<Rightarrow> 'a Rules option" where
   "find_common m (m' ? r) = (if m = m' then Some r else None)" |
@@ -471,8 +950,135 @@ fun find_uncommon :: "'a::Rewritable MATCH \<Rightarrow> 'a Rules \<Rightarrow> 
 definition join_common :: "'a::Rewritable MATCH \<Rightarrow> 'a Rules list \<Rightarrow> 'a Rules list" where
   "join_common m rules = List.map_filter (find_common m) rules"
 
+lemma find_common_defn:
+  assumes "find_common m x = v"
+  shows "v \<noteq> None \<longleftrightarrow> (\<exists>r. x = (m ? r) \<and> v = Some r)"
+  using assms apply (induction m x rule: find_common.induct) unfolding find_common.simps apply force
+  by simp+
+
+lemma find_common_shrinks:
+  "find_common m x = Some z \<Longrightarrow> common_size z \<le> common_size x"
+  unfolding find_common.simps using find_common_defn
+  by (metis common_size.simps(1) le_add2 option.distinct(1) option.inject)
+
+lemma join_common_shrinks:
+  "common_size (choice (join_common m x)) \<le> common_size (choice x)"
+  unfolding join_common_def
+  apply (induction x)
+   apply (simp add: map_filter_simps(2))
+  subgoal for a x
+    apply (cases "find_common m a") unfolding List.map_filter_def apply simp
+    using find_common_shrinks apply simp
+    using add_le_mono by blast
+  done
+
 definition join_uncommon :: "'a::Rewritable MATCH \<Rightarrow> 'a Rules list \<Rightarrow> 'a Rules list" where
   "join_uncommon m rules = List.map_filter (find_uncommon m) rules"
+
+lemma find_uncommon_preserve:
+  "find_uncommon m r = Some r \<or> find_uncommon m r = None"
+  by (metis find_uncommon.elims)
+
+lemma join_uncommon_subset:
+  "set (join_uncommon m x) \<subseteq> set x"
+  unfolding join_uncommon_def List.map_filter_def using find_uncommon_preserve
+  by (smt (verit, best) comp_def filter_is_subset list.map_ident_strong mem_Collect_eq option.sel set_filter)
+
+lemma size_join_uncommon:
+  "\<forall>r \<in> set (join_uncommon m rules) . find_uncommon m r = Some r' \<longrightarrow> common_size r' \<le> common_size r"
+  unfolding join_uncommon_def map_filter_def
+  apply (induction rule: find_uncommon.induct; auto) 
+  apply (metis common_size.simps(1) dual_order.eq_iff find_uncommon_preserve option.distinct(1) option.sel plus_1_eq_Suc)
+    apply (metis Suc_eq_plus1_left add_Suc_right add_Suc_shift common_size.simps(3) find_uncommon_preserve option.distinct(1) option.inject order_refl)
+  apply (metis Suc_eq_plus1_left add_Suc_right add_Suc_shift common_size.simps(6) find_uncommon_preserve le_refl option.distinct(1) option.inject)
+  by (metis find_uncommon_preserve option.distinct(1) option.inject verit_comp_simplify1(2))
+
+lemma find_uncommon_shrinks:
+  "find_uncommon m x = Some z \<Longrightarrow> common_size z \<le> common_size x"
+  unfolding find_uncommon.simps
+  by (metis dual_order.refl find_uncommon_preserve option.distinct(1) option.inject)
+
+lemma join_uncommon_shrinks:
+  "common_size (choice (join_uncommon m rules))
+       \<le> (common_size (choice rules))"
+  unfolding join_uncommon_def
+  apply (induction rules)
+   apply (simp add: map_filter_simps(2))
+  subgoal for a x
+    apply (cases "find_uncommon m a") unfolding List.map_filter_def apply simp
+    using find_uncommon_shrinks
+    by fastforce
+  done
+
+lemma join_common_empty: "join_common m [] = []"
+  by (simp add: join_common_def map_filter_simps(2))
+lemma join_uncommon_empty: "join_uncommon m [] = []"
+  by (simp add: join_uncommon_def map_filter_simps(2))
+
+lemma find_inverse_lhs:
+  "\<exists>e. find_common m rules = None \<longleftrightarrow> find_uncommon m rules = Some e"
+  by (smt (verit, best) find_common.elims find_uncommon.simps(1) find_uncommon.simps(2) find_uncommon.simps(3) find_uncommon.simps(4) find_uncommon.simps(5))
+
+lemma find_inverse_rhs:
+  "\<exists>e. find_common m rules = Some e \<longleftrightarrow> find_uncommon m rules = None"
+  by (smt (verit, best) find_common.elims find_uncommon.simps(1) find_uncommon.simps(2) find_uncommon.simps(3) find_uncommon.simps(4) find_uncommon.simps(5))
+
+lemma join_common_equal:
+  assumes "find_common m a = None"
+  shows "(map ((?) m) (join_common m rules')) = (map ((?) m) (join_common m (a # rules')))"
+  apply (simp add: join_common_def join_uncommon_def List.map_filter_def)
+  by (simp add: assms)
+
+lemma join_common_plus:
+  assumes "find_common m a = Some a'"
+  shows "(m ? a') # (map ((?) m) (join_common m rules')) = (map ((?) m) (join_common m (a # rules')))"
+  using assms unfolding join_common_def join_uncommon_def List.map_filter_def
+  by simp
+
+
+lemma join_combines:
+  "(set (map (\<lambda>r. m ? r) (join_common m rules)) \<union> set (join_uncommon m rules)) = set rules"
+  apply (induction rules) 
+    apply (simp add: join_common_def join_uncommon_def List.map_filter_def)
+  subgoal premises induct for a rules'
+  proof (cases "find_common m a")
+    case None
+    have "find_uncommon m a = Some a" 
+      using None find_inverse_lhs
+      by (metis find_uncommon_preserve option.distinct(1))
+    then have "join_uncommon m (a # rules') = a # (join_uncommon m rules')"
+      unfolding join_common_def join_uncommon_def List.map_filter_def
+      by simp
+    then show ?thesis using induct join_common_equal
+      by (metis None Un_insert_right list.simps(15))
+  next
+    case (Some a')
+    have "find_uncommon m a = None" 
+      by (metis Some find_common_defn find_uncommon.simps(1) option.distinct(1))
+    then have "join_uncommon m (a # rules') = (join_uncommon m rules')"
+      unfolding join_common_def join_uncommon_def List.map_filter_def
+      by simp
+    then show ?thesis
+      by (metis Some Un_insert_left find_common.elims induct join_common_plus list.simps(15) option.distinct(1))
+  qed
+  done
+
+lemma join_common_set_def:
+  "set (join_common m rules) = {r. (m ? r) \<in> set rules}"
+  unfolding join_common_def List.map_filter_def 
+  apply (induction rules)
+   apply simp 
+  subgoal for a rules 
+    apply (cases a) by auto
+  done
+
+lemma join_uncommon_set_def:
+  "set (join_uncommon m rules) = {r. r \<in> set rules \<and> (\<forall>r'. r \<noteq> (m ? r'))}"
+  unfolding join_uncommon_def List.map_filter_def 
+  apply (induction rules) apply simp
+  subgoal for a rules 
+    apply (cases a) by auto
+  done
 
 function (sequential) combine_conditions :: "'a::Rewritable Rules \<Rightarrow> 'a Rules" where
   "combine_conditions (base e) = base e" |
@@ -487,7 +1093,239 @@ function (sequential) combine_conditions :: "'a::Rewritable Rules \<Rightarrow> 
   apply pat_completeness+
   by simp+
 
-termination combine_conditions sorry
+lemma find_common_size:
+  assumes "(find_common m r) \<noteq> None"
+  shows "size (the (find_common m r)) < size r"
+  using assms apply (induction r rule: find_common.induct)
+  apply simp+ apply fastforce by simp+
+
+lemma common_size_choice_gt:
+  "x \<in> set va \<Longrightarrow> common_size x \<le> common_size (choice va)"
+  apply (induction va) apply simp
+  by fastforce
+
+termination combine_conditions
+  apply (relation "measures [common_size]") apply auto[1] apply simp+ using join_common_shrinks
+  using le_imp_less_Suc apply blast
+          apply (simp add: le_imp_less_Suc) defer
+         apply simp apply auto[1]
+        apply (simp add: common_size_choice_gt le_imp_less_Suc)
+       apply auto[1] using common_size_choice_gt apply fastforce
+      apply auto[1] using common_size_choice_gt apply fastforce
+     apply auto[1] using common_size_choice_gt apply fastforce
+    apply simp+ using join_uncommon_shrinks
+  by (metis le_imp_less_Suc plus_1_eq_Suc trans_le_add2)
+
+lemma cases_None:
+  assumes "eval_rules (choice ((m ? r) # rules)) u None"
+  shows "
+  eval_rules (m ? (choice (r # join_common m rules))) u None \<and>
+  eval_rules ((choice (join_uncommon m rules))) u None"
+  apply (rule conjI)
+  using assms
+  unfolding join_common_def List.map_filter_def
+   apply (induction rules) apply simp using pull_cond_out
+    apply fastforce apply auto[1] using pull_cond_out defer defer
+    apply (meson assms eval_choice_none join_uncommon_subset list.set_intros(2) subsetD)
+  subgoal for a rules y
+    apply (cases a)
+        apply force
+    subgoal premises pre for m' r' 
+    proof -
+      have "m = m'"
+        using pre(3,4)
+        by (metis find_common.simps(1) option.distinct(1))
+      then show ?thesis using pre apply auto[1]
+        by (smt (verit, del_insts) eval_choice_none list.set_intros(1) list.set_intros(2) list.simps(9) pull_cond_out set_ConsD)
+    qed
+      by simp+
+  subgoal for a rules
+    apply (cases a)
+    by (simp add: eval_choice_none)+
+  done
+
+lemma cases_None1:
+  assumes "
+  eval_rules (m ? (choice (r # join_common m rules))) u None \<and>
+  eval_rules ((choice (join_uncommon m rules))) u None"
+  shows "eval_rules (choice ((m ? r) # rules)) u None"
+proof -
+  have head: "eval_rules (m ? r) u None"
+    using assms
+    by (meson list.set_intros(1) map_None pull_cond_out_lhs)
+  have common_None: "\<forall>r' \<in> set (join_common m rules). eval_rules (m ? r') u None"
+    by (meson assms list.set_intros(2) map_None pull_cond_out_lhs)
+  have uncommon_None: "\<forall>r' \<in> set (join_uncommon m rules). eval_rules r' u None"
+    using assms eval_choice_none by blast
+  have "\<forall>r' \<in> set rules. eval_rules r' u None"
+    using join_combines common_None uncommon_None pull_cond_out
+    by (metis (no_types, lifting) UnE assms eval_choice_none list.set_intros(2) list.simps(9))
+  then show ?thesis using head
+    by (simp add: eval_choice_none)
+qed
+
+  
+lemma cases_Some:
+  assumes "eval_rules (choice rules) u (Some e)"
+  shows "
+  eval_rules (m ? (choice (join_common m rules))) u (Some e) \<or>
+  eval_rules ((choice (join_uncommon m rules))) u (Some e)"
+proof -
+  obtain r where r: "r \<in> set rules \<and> eval_rules r u (Some e)"
+    by (metis assms choiceE option.discI)
+  then show ?thesis
+  proof (cases r)
+    case (base x1)
+    have "r \<in> set (join_uncommon m rules)"
+      using join_uncommon_set_def base r by blast
+    then show ?thesis
+      using eval_rules.intros(6) r by blast
+  next
+    case (cond m' r')
+    then show ?thesis
+    proof (cases "m = m'")
+      case True
+      then have "r' \<in> set (join_common m rules)"
+        using cond r join_common_set_def
+        by blast
+      then show ?thesis
+        by (metis True cond eval_rules.intros(6) image_eqI image_set pull_cond_out_rhs r)
+    next
+      case False
+      have "r \<in> set (join_uncommon m rules)"
+        using join_uncommon_set_def False r
+        using cond by blast
+      then show ?thesis
+        using eval_rules.intros(6) r by blast
+    qed
+  next
+    case (else x31 x32)
+    have "r \<in> set (join_uncommon m rules)"
+      using join_uncommon_set_def else r by blast
+    then show ?thesis
+      using eval_rules.intros(6) r by blast
+  next
+    case (seq x41 x42)
+    have "r \<in> set (join_uncommon m rules)"
+      using join_uncommon_set_def seq r by blast
+    then show ?thesis
+      using eval_rules.intros(6) r by blast
+  next
+    case (choice x5)
+    have "r \<in> set (join_uncommon m rules)"
+      using join_uncommon_set_def choice r by blast
+    then show ?thesis
+      using eval_rules.intros(6) r by blast
+  qed
+qed
+
+lemma cases_Some1:
+  assumes "eval_rules (choice ((m ? r) # rules)) u (Some e)"
+  shows "
+  eval_rules (m ? (choice (r # join_common m rules))) u (Some e) \<or>
+  eval_rules ((choice (join_uncommon m rules))) u (Some e)"
+  using cases_Some assms
+  by (smt (verit, ccfv_threshold) choiceE eval_rules.intros(6) list.set_intros(1) list.set_intros(2) list.simps(9) option.distinct(1) pull_cond_out set_ConsD)
+
+lemma cases_Some2:
+  assumes "eval_rules (m ? (choice (r # join_common m rules))) u (Some e) \<or>
+  eval_rules ((choice (join_uncommon m rules))) u (Some e)" (is "?c1 \<or> ?c2")
+  shows "eval_rules (choice ((m ? r) # rules)) u (Some e)"
+using assms proof (rule disjE)
+  assume c1: "?c1"
+  then show ?thesis
+  proof (cases "eval_rules (m ? r) u (Some e)")
+    case True
+    then show ?thesis
+      by (meson eval_rules.intros(6) list.set_intros(1))
+  next
+    case False
+    then have "\<exists>r \<in>set (join_common m rules). eval_rules (m ? r) u (Some e)"
+      using c1
+      by (smt (verit, del_insts) choiceE condE eval_rules.intros(2) option.distinct(1) set_ConsD)
+    then show ?thesis 
+      by (metis eval_rules.intros(6) join_common_set_def list.set_intros(2) mem_Collect_eq)
+  qed
+next
+  assume "?c2"
+  then have "\<exists>r \<in>set (join_uncommon m rules). eval_rules r u (Some e)"
+    by (metis choiceE option.discI)
+  then show ?thesis
+    by (meson eval_rules.intros(6) join_uncommon_subset list.set_intros(2) subsetD)
+qed
+
+lemma evalchoice_twoelement:
+  assumes "eval_rules (choice [x1, x2]) u (Some e)"
+  shows "eval_rules x1 u (Some e) \<or> eval_rules x2 u (Some e)"
+  using assms choiceE by fastforce
+
+lemma combine_conditions_valid:
+  "eval_rules r u e = eval_rules (combine_conditions r) u e"
+  apply (induction r arbitrary: u e rule: combine_conditions.induct) apply simp
+  apply (simp add: monotonic)+
+        defer
+  apply simp+
+  apply (metis (mono_tags, lifting) choice_join combine_conditions.simps(1) list.simps(9) monotonic_choice)
+  using monotonic_choice
+  using combine_conditions.simps(7) monotonic_choice apply metis
+  using combine_conditions.simps(8) monotonic_choice apply metis
+  using combine_conditions.simps(9) monotonic_choice apply metis
+   apply (simp add: monotonic)+
+  subgoal premises p for m r rules u e
+  proof (rule iffI)
+    assume eval: "eval_rules (choice ((m ? r) # rules)) u e"
+    show "eval_rules
+     (choice
+       [m ? combine_conditions (choice (r # join_common m rules)),
+        combine_conditions (choice (join_uncommon m rules))])
+     u e"
+    proof (cases e)
+      case None
+      have "eval_rules (m ? (choice (r # join_common m rules))) u None \<and>
+  eval_rules ((choice (join_uncommon m rules))) u None"
+        using None cases_None eval by blast
+      then have "eval_rules (m ? combine_conditions (choice (r # join_common m rules))) u None \<and>
+  eval_rules (combine_conditions (choice (join_uncommon m rules))) u None" 
+        using p monotonic_cond by blast
+      then show ?thesis using None eval_choice_none by fastforce
+    next
+      case (Some a)
+      have "eval_rules (m ? (choice (r # join_common m rules))) u (Some a) \<or>
+  eval_rules ((choice (join_uncommon m rules))) u (Some a)"
+        using Some cases_Some1 eval by simp
+      then have "eval_rules (m ? combine_conditions (choice (r # join_common m rules))) u (Some a) \<or>
+  eval_rules (combine_conditions (choice (join_uncommon m rules))) u (Some a)"
+        using p monotonic_cond by blast
+      then show ?thesis
+        by (metis Some eval_rules.intros(6) list.set_intros(1) list.set_intros(2))
+    qed
+  next
+    assume eval: "eval_rules
+     (choice
+       [m ? combine_conditions (choice (r # join_common m rules)),
+        combine_conditions (choice (join_uncommon m rules))])
+     u e"
+    show "eval_rules (choice ((m ? r) # rules)) u e"
+    proof (cases e)
+      case None
+      then have "eval_rules (m ? (choice (r # join_common m rules))) u None \<and>
+  eval_rules ((choice (join_uncommon m rules))) u None"
+        by (smt (verit) eval eval_choice_none list.set_intros(1) list.set_intros(2) monotonic_cond p(1) p(2))
+      then show ?thesis using cases_None1 None by blast
+    next
+      case (Some a)
+      then have "eval_rules (m ? combine_conditions (choice (r # join_common m rules))) u (Some a) \<or>
+  eval_rules (combine_conditions (choice (join_uncommon m rules))) u (Some a)"
+        using eval evalchoice_twoelement by simp
+      then have "eval_rules (m ? (choice (r # join_common m rules))) u (Some a) \<or>
+  eval_rules ((choice (join_uncommon m rules))) u (Some a)"
+        using p monotonic_cond by blast
+      then show ?thesis using cases_Some2 Some
+        by simp
+    qed
+  qed
+  done
+
 
 fun eliminate_choice :: "'a::Rewritable Rules \<Rightarrow> 'a Rules" where
   "eliminate_choice (base e) = base e" |
@@ -498,9 +1336,97 @@ fun eliminate_choice :: "'a::Rewritable Rules \<Rightarrow> 'a Rules" where
     choice (List.map eliminate_choice rules)" |
   "eliminate_choice (r1 \<then> r2) = (eliminate_choice r1 \<then> eliminate_choice r2)"
 
-definition optimized_export where
-  "optimized_export = eliminate_choice \<circ> combine_conditions o lift_common o lift_match o eliminate_noop o eliminate_empty"
+lemma eliminate_choice_valid_1:
+  "{e. eval_rules r u e} = {e. eval_rules (eliminate_choice r) u e}"
+  apply (induction r arbitrary: u rule: eliminate_choice.induct)
+  apply simp unfolding eliminate_choice.simps
+  apply (smt (verit) Collect_cong elseE eval_rules.intros(4) eval_rules.intros(5) mem_Collect_eq)
+  unfolding eliminate_choice.simps
+  apply (metis (mono_tags) Collect_cong mem_Collect_eq monotonic_cond)
+  unfolding eliminate_choice.simps
+  using choice_Single apply blast
+  using monotonic_choice apply blast
+  apply (metis Collect_cong mem_Collect_eq monotonic_choice)
+  by (smt (verit) Collect_cong eval_rules.intros(10) eval_rules.intros(9) mem_Collect_eq seqE)
 
+lemma eliminate_choice_valid:
+  "eval_rules r u e = eval_rules (eliminate_choice r) u e"
+  using eliminate_choice_valid_1 by blast
+
+definition optimized_export where
+  "optimized_export = eliminate_choice \<circ> combine_conditions o lift_common o lift_match o eliminate_noop"
+
+
+(*lemma elim_empty_preserve_def_vars:
+  "def_vars m = def_vars (elim_empty m)"
+  apply (induction m rule: elim_empty.induct) by simp+
+
+lemma elim_empty_preserve_use_vars:
+  "use_vars m = use_vars (elim_empty m)"
+  apply (induction m rule: elim_empty.induct) apply simp
+  using elim_empty_preserve_def_vars apply auto[1] by simp+
+
+lemma elim_empty_preserve_valid:
+  assumes "valid_match m"
+  shows "valid_match (elim_empty m)"
+    using assms apply (induction m rule: elim_empty.induct) apply simp
+    using elim_empty_preserve_def_vars elim_empty_preserve_use_vars apply auto[1] 
+    by simp+
+
+lemma eliminate_empty_preserve_valid:
+  assumes "valid_rules r"
+  shows "valid_rules (eliminate_empty r)"
+  using assms apply (induction r rule: eliminate_empty.induct) apply simp
+  apply (simp add: elim_empty_preserve_valid) by simp+*)
+
+lemma elim_noop_preserve_def_vars:
+  "def_vars m = def_vars (elim_noop m)"
+  apply (induction m rule: elim_noop.induct) by simp+
+
+lemma elim_noop_preserve_use_vars:
+  "use_vars m = use_vars (elim_noop m)"
+  apply (induction m rule: elim_noop.induct) apply simp+
+  using def_vars.simps(3) elim_noop_preserve_def_vars apply blast
+  apply simp+
+  using def_vars.simps(3) elim_noop_preserve_def_vars apply blast
+  by simp+
+
+lemma elim_noop_preserve_valid:
+  assumes "valid_match m"
+  shows "valid_match (elim_noop m)"
+  using assms apply (induction m rule: elim_noop.induct) apply simp+
+  using elim_noop_preserve_use_vars
+  apply (metis use_vars.simps(3))
+  apply simp+
+  apply (metis DiffE UnE elim_noop_preserve_use_vars use_vars.simps(3))
+  apply simp
+  apply (metis elim_noop.simps(14) elim_noop.simps(22) elim_noop_preserve_def_vars valid_match.simps(2))
+  apply simp
+  apply (metis (no_types, lifting) elim_noop.simps(16) elim_noop_preserve_def_vars elim_noop_preserve_use_vars valid_match.simps(2))
+  by simp+
+
+lemma eliminate_noop_preserve_valid:
+  assumes "valid_rules r"
+  shows "valid_rules (eliminate_noop r)"
+  using assms apply (induction r rule: eliminate_noop.induct) apply simp
+  apply (simp add: elim_noop_preserve_valid) by simp+
+
+
+lemma lift_match_preserve_valid:
+  assumes "valid_rules r"
+  shows "valid_rules (lift_match r)"
+  using assms apply (induction r rule: lift_match.induct) apply simp
+  by simp+
+
+lemma optimized_export_valid:
+  assumes "valid_rules r"
+  shows "eval_rules r u e = eval_rules (optimized_export r) u e"
+  unfolding optimized_export_def comp_def
+  using lift_match_valid eliminate_noop_valid 
+  using combine_conditions_valid eliminate_choice_valid
+  by (metis assms eliminate_noop_preserve_valid lift_common_valid lift_match_preserve_valid)
+
+thm_oracles optimized_export_valid
 
 value "optimized_export
 (generate
